Fix initial states and RTLtyping
We need to actually use the provided arguments in the initial state,
and make sure that their types match the function signature.

backend/Cminor.v
@@ -559,7 +559,8 @@ Inductive initial_state (p: program): query li_c -> state -> Prop :=
       Ple (Genv.genv_next ge) (Mem.nextblock m) ->
       Genv.find_symbol ge (str2ident id) = Some b ->
       Genv.find_funct_ptr ge b = Some f ->
-      initial_state p (id, funsig f, vargs, m) (Callstate f nil Kstop m).
+      Val.has_type_list vargs (sig_args (funsig f)) ->
+      initial_state p (id, funsig f, vargs, m) (Callstate f vargs Kstop m).
 
 (** A final state is a [Returnstate] with an empty continuation. *)
 
@@ -839,7 +840,8 @@ Inductive bigstep_program_terminates (p: program):
       Ple (Genv.genv_next ge) (Mem.nextblock m0) ->
       Genv.find_symbol ge (str2ident id) = Some b ->
       Genv.find_funct_ptr ge b = Some f ->
-      eval_funcall ge m0 f nil t m r ->
+      Val.has_type_list vargs (sig_args (funsig f)) ->
+      eval_funcall ge m0 f vargs t m r ->
       bigstep_program_terminates p (id, funsig f, vargs, m0) t (r, m).
 
 Inductive bigstep_program_diverges (p: program):
@@ -850,7 +852,8 @@ Inductive bigstep_program_diverges (p: program):
       Ple (Genv.genv_next ge) (Mem.nextblock m0) ->
       Genv.find_symbol ge (str2ident id) = Some b ->
       Genv.find_funct_ptr ge b = Some f ->
-      evalinf_funcall ge m0 f nil t ->
+      Val.has_type_list vargs (sig_args (funsig f)) ->
+      evalinf_funcall ge m0 f vargs t ->
       bigstep_program_diverges p (id, funsig f, vargs, m0) t.
 
 Definition bigstep_semantics (p: program) :=
